Add doc comments to PossiblyInfiniteTree

PossiblyInfiniteTrees/PossiblyInfiniteTree/PossiblyInfiniteTree.lean
@@ -1,8 +1,20 @@
 import PossiblyInfiniteTrees.PossiblyInfiniteTree.InfiniteTree
 
+/-!
+# PossiblyInfiniteTree
+
+This file defines a `PossiblyInfiniteTree` which is an `InfiniteTreeSkeleton` over an `Option` of the desired type.
+The offered functions are similar to the ones of `InfiniteTreeSkeleton`.
+The tree can still be infinite in both dimensions, i.e.
+it may have infinite depth and each node may have infinitely many (direct) children.
+-/
+
+
+/-- An `InfiniteTreeSkeleton` over `Option` has `no_orphans` if an element being `none` implies its `InfiniteTreeSkeleton.childNodes` also being `none`. That is, intuitively, every non-none node needs to have a non-none parent. This is a property that we want for possibly infinite trees but we need to be able to express it on the underlying infinite tree first. -/
 def InfiniteTreeSkeleton.no_orphans (t : InfiniteTreeSkeleton (Option α)) : Prop :=
   ∀ ns : List Nat, t.get ns = none -> ∀ n, (t.drop ns).childNodes.get n = none
 
+/-- A closed version of the `no_orphans` property. That is, if an element is none, then not only its immediate childNodes but all nodes in all subtrees are none. -/
 theorem InfiniteTreeSkeleton.no_orphans_closure {t : InfiniteTreeSkeleton (Option α)} (no_orph : t.no_orphans) :
     ∀ ns : List Nat, t.get ns = none -> ∀ ns', (t.drop ns).get ns' = none := by
   intro ns eq_none ns'
@@ -17,6 +29,7 @@ theorem InfiniteTreeSkeleton.no_orphans_closure {t : InfiniteTreeSkeleton (Optio
     rw [get_drop]
     exact ih
 
+/-- A `PossiblyInfiniteTree` is an `InfiniteTreeSkeleton` over `Option` that has `no_orphans` and also for each subtree, its `InfiniteTreeSkeleton.childNodes` have `InfiniteList.no_holes`. The last condition is necessary because we want the trees to be somewhat "compact", meaning that we want to forbid that e.g. the second child for a node is defined but the first child is none. Note that this would not be captured by the `InfiniteTreeSkeleto.no_orphans` property yet. -/
 structure PossiblyInfiniteTree (α : Type u) where
   infinite_tree : InfiniteTreeSkeleton (Option α)
   no_orphans : infinite_tree.no_orphans
@@ -24,551 +37,750 @@ structure PossiblyInfiniteTree (α : Type u) where
 
 namespace PossiblyInfiniteTree
 
-  def empty : PossiblyInfiniteTree α where
-    infinite_tree := fun _ => none
-    no_orphans := by intro _ _ _; rw [InfiniteTreeSkeleton.get_childNodes, InfiniteTreeSkeleton.get_drop]; simp [InfiniteTreeSkeleton.get]
-    no_holes_in_children := by rintro _ ⟨_, eq⟩ _ _; rw [← eq, InfiniteTreeSkeleton.get_childNodes, InfiniteTreeSkeleton.get_drop]; simp [InfiniteTreeSkeleton.get]
+section Basic
 
-  def get? (t : PossiblyInfiniteTree α) (ns : List Nat) : Option α := t.infinite_tree.get ns
+/-!
+## Basics
 
-  theorem get?_empty {α} : ∀ {n}, (@PossiblyInfiniteTree.empty α).get? n = none := by intro _; rfl
+The essential functions on infinite trees, mainly get, drop, and root.
+The `childTrees` function is defined separately here since it is more involved than for the `InfiniteTreeSkeleton` case.
+-/
 
-  instance : Membership α (PossiblyInfiniteTree α) where
-    mem t a := some a ∈ t.infinite_tree
+/-- Obtains the element of the tree at the given address. -/
+def get? (t : PossiblyInfiniteTree α) (ns : List Nat) : Option α := t.infinite_tree.get ns
 
-  theorem mem_iff {t : PossiblyInfiniteTree α} : ∀ {e}, e ∈ t ↔ ∃ ns, t.get? ns = some e := by rfl
+/-- Obtains the subtree at the given address (by dropping everything else). -/
+def drop (t : PossiblyInfiniteTree α) (ns : List Nat) : PossiblyInfiniteTree α where
+  infinite_tree := t.infinite_tree.drop ns
+  no_orphans := by intro ns'; rw [InfiniteTreeSkeleton.get_drop]; intro eq_none n; rw [InfiniteTreeSkeleton.drop_drop]; apply t.no_orphans; exact eq_none
+  no_holes_in_children := by intro _ suf; apply t.no_holes_in_children; exact InfiniteTreeSkeleton.IsSuffix_trans suf (t.infinite_tree.IsSuffix_drop ns)
 
-  def Element (t : PossiblyInfiniteTree α) := { e : α // e ∈ t }
+/-- Get the element at the root of the tree (i.e. at the empty address). -/
+def root (t : PossiblyInfiniteTree α) : Option α := t.infinite_tree.root
 
-  def drop (t : PossiblyInfiniteTree α) (ns : List Nat) : PossiblyInfiniteTree α where
-    infinite_tree := t.infinite_tree.drop ns
-    no_orphans := by intro ns'; rw [InfiniteTreeSkeleton.get_drop]; intro eq_none n; rw [InfiniteTreeSkeleton.drop_drop]; apply t.no_orphans; exact eq_none
-    no_holes_in_children := by intro _ suf; apply t.no_holes_in_children; exact InfiniteTreeSkeleton.IsSuffix_trans suf (t.infinite_tree.IsSuffix_drop ns)
+instance : Membership α (PossiblyInfiniteTree α) where
+  mem t a := some a ∈ t.infinite_tree
 
-  -- inspired by List.IsSuffix; see https://github.com/leanprover/lean4/blob/9d4ad1273f6cea397c3066c2c83062a4410d16bf/src/Init/Data/List/Basic.lean#L1205
-  def IsSuffix (t1 t2 : PossiblyInfiniteTree α) : Prop := t1.infinite_tree <:+ t2.infinite_tree
-  infixl:50 " <:+ " => IsSuffix
+/-- An element is a member of the tree iff it occurs at some address. -/
+theorem mem_iff {t : PossiblyInfiniteTree α} : ∀ {e}, e ∈ t ↔ ∃ ns, t.get? ns = some e := by rfl
 
-  theorem IsSuffix_iff {t1 t2 : PossiblyInfiniteTree α} : t1 <:+ t2 ↔ ∃ ns, t2.drop ns = t1 := by
-    constructor
-    . rintro ⟨ns, h⟩; exists ns; simp [drop, h]
-    . rintro ⟨ns, h⟩; exists ns; simp only [drop] at h; rw [← h]
+/-- Two `PossiblyInfiniteTree`s are the same if they agree on all addresses. -/
+theorem ext {t1 t2 : PossiblyInfiniteTree α} : (∀ ns, t1.get? ns = t2.get? ns) -> t1 = t2 := by
+  intro h; rw [PossiblyInfiniteTree.mk.injEq]; apply InfiniteTreeSkeleton.ext; exact h
 
-  theorem drop_nil {t : PossiblyInfiniteTree α} : t.drop [] = t := by rfl
+theorem ext_iff {t1 t2 : PossiblyInfiniteTree α} : t1 = t2 ↔ (∀ ns, t1.get? ns = t2.get? ns) := by
+  constructor
+  . intro h _; rw [h]
+  . exact ext
 
-  theorem get?_drop {t : PossiblyInfiniteTree α} {ns ns' : List Nat} : (t.drop ns).get? ns' = t.get? (ns ++ ns') := by rfl
+/-- Get after drop can be rewritten into get. -/
+theorem get?_drop {t : PossiblyInfiniteTree α} {ns ns' : List Nat} : (t.drop ns).get? ns' = t.get? (ns ++ ns') := by rfl
 
-  theorem drop_drop {t : PossiblyInfiniteTree α} {ns ns' : List Nat} : (t.drop ns).drop ns' = t.drop (ns ++ ns') := by simp [drop, InfiniteTreeSkeleton.drop_drop]
+/-- Dropping the empty address changes nothing. -/
+theorem drop_nil {t : PossiblyInfiniteTree α} : t.drop [] = t := by rfl
 
-  theorem mem_of_mem_suffix {t1 t2 : PossiblyInfiniteTree α} (suffix : t1 <:+ t2) : ∀ e ∈ t1, e ∈ t2 := by
-    intro e mem; apply InfiniteTreeSkeleton.mem_of_mem_suffix suffix; exact mem
+/-- Two calls to drop can be combined. -/
+theorem drop_drop {t : PossiblyInfiniteTree α} {ns ns' : List Nat} : (t.drop ns).drop ns' = t.drop (ns ++ ns') := by simp [drop, InfiniteTreeSkeleton.drop_drop]
 
-  theorem ext {t1 t2 : PossiblyInfiniteTree α} : (∀ ns, t1.get? ns = t2.get? ns) -> t1 = t2 := by
-    intro h; rw [PossiblyInfiniteTree.mk.injEq]; apply InfiniteTreeSkeleton.ext; exact h
+/-- The `root` is equal to getting the empty address. -/
+theorem root_eq {t : PossiblyInfiniteTree α} : t.root = t.get? [] := by rfl
 
-  theorem ext_iff {t1 t2 : PossiblyInfiniteTree α} : t1 = t2 ↔ (∀ ns, t1.get? ns = t2.get? ns) := by
-    constructor
-    . intro h _; rw [h]
-    . exact ext
+/-- The root is in the tree. -/
+theorem root_mem {t : PossiblyInfiniteTree α} : ∀ r ∈ t.root, r ∈ t := by intro h h_mem; rw [Option.mem_def] at h_mem; simp only [Membership.mem, ← h_mem]; exact t.infinite_tree.root_mem
 
-  theorem drop_empty {α} : ∀ {ns}, (@PossiblyInfiniteTree.empty α).drop ns = PossiblyInfiniteTree.empty := by
-    intro _; apply ext; intro _; rw [get?_drop, get?_empty, get?_empty]
+/-- The root of the dropped tree at address ns is exactly the element at address ns. -/
+theorem root_drop {t : PossiblyInfiniteTree α} {ns : List Nat} : (t.drop ns).root = t.get? ns := by
+  unfold root drop; simp [InfiniteTreeSkeleton.root_drop]; rfl
 
-  theorem IsSuffix_refl {t : PossiblyInfiniteTree α} : t <:+ t := t.infinite_tree.IsSuffix_refl
+end Basic
 
-  theorem IsSuffix_drop {t : PossiblyInfiniteTree α} : ∀ ns, t.drop ns <:+ t := t.infinite_tree.IsSuffix_drop
+section Empty
 
-  theorem IsSuffix_trans {t1 t2 t3 : PossiblyInfiniteTree α} : t1 <:+ t2 -> t2 <:+ t3 -> t1 <:+ t3 := InfiniteTreeSkeleton.IsSuffix_trans
+/-!
+## Empty Infinite Trees
 
-  def root (t : PossiblyInfiniteTree α) : Option α := t.infinite_tree.root
+The `empty` `PossiblyInfiniteTree` is simply the `PossiblyInfiniteTree` that is `none` on all addresses.
+-/
 
-  theorem root_mem {t : PossiblyInfiniteTree α} : ∀ r ∈ t.root, r ∈ t := by intro h h_mem; rw [Option.mem_def] at h_mem; simp only [Membership.mem, ← h_mem]; exact t.infinite_tree.root_mem
+/-- The empty `PossiblyInfiniteTree` is none everywhere. -/
+def empty : PossiblyInfiniteTree α where
+  infinite_tree := fun _ => none
+  no_orphans := by intro _ _ _; rw [InfiniteTreeSkeleton.get_childNodes, InfiniteTreeSkeleton.get_drop]; simp [InfiniteTreeSkeleton.get]
+  no_holes_in_children := by rintro _ ⟨_, eq⟩ _ _; rw [← eq, InfiniteTreeSkeleton.get_childNodes, InfiniteTreeSkeleton.get_drop]; simp [InfiniteTreeSkeleton.get]
 
-  theorem root_eq {t : PossiblyInfiniteTree α} : t.root = t.get? [] := by rfl
+/-- Getting from the `empty` tree always returns none. -/
+theorem get?_empty {α} : ∀ {n}, (@PossiblyInfiniteTree.empty α).get? n = none := by intro _; rfl
 
-  theorem root_drop {t : PossiblyInfiniteTree α} {ns : List Nat} : (t.drop ns).root = t.get? ns := by
-    unfold root drop; simp [InfiniteTreeSkeleton.root_drop]; rfl
+/-- Dropping from the `empty` tree again yields the empty tree. -/
+theorem drop_empty {α} : ∀ {ns}, (@PossiblyInfiniteTree.empty α).drop ns = PossiblyInfiniteTree.empty := by
+  intro _; apply ext; intro _; rw [get?_drop, get?_empty, get?_empty]
 
-  theorem root_empty {α} : (@PossiblyInfiniteTree.empty α).root = none := by rfl
+/-- The `root` of the `empty` tree is none. -/
+theorem root_empty {α} : (@PossiblyInfiniteTree.empty α).root = none := by rfl
 
-  theorem empty_iff_root_none {t : PossiblyInfiniteTree α} : t = PossiblyInfiniteTree.empty ↔ t.root = none := by
-    constructor
-    . intro h; rw [h]; exact root_empty
-    intro h
-    rw [root_eq] at h
-    apply PossiblyInfiniteTree.ext
-    intro ns
-    induction ns generalizing t with
-    | nil => rw [h]; rfl
-    | cons n ns ih =>
-      rw [← List.singleton_append, ← get?_drop];
-      rw [ih]
-      . rfl
-      . rw [get?_drop]
-        have := t.no_orphans [] h n
-        rw [InfiniteTreeSkeleton.get_childNodes, InfiniteTreeSkeleton.get_drop] at this
-        exact this
+/-- A tree is `empty` if and only if the `root` is none. -/
+theorem empty_iff_root_none {t : PossiblyInfiniteTree α} : t = PossiblyInfiniteTree.empty ↔ t.root = none := by
+  constructor
+  . intro h; rw [h]; exact root_empty
+  intro h
+  rw [root_eq] at h
+  apply PossiblyInfiniteTree.ext
+  intro ns
+  induction ns generalizing t with
+  | nil => rw [h]; rfl
+  | cons n ns ih =>
+    rw [← List.singleton_append, ← get?_drop];
+    rw [ih]
+    . rfl
+    . rw [get?_drop]
+      have := t.no_orphans [] h n
+      rw [InfiniteTreeSkeleton.get_childNodes, InfiniteTreeSkeleton.get_drop] at this
+      exact this
 
-  abbrev PossiblyInfiniteTreeWithRoot (α : Type u) := {t : PossiblyInfiniteTree α // t.root ≠ none}
+end Empty
 
-  namespace PossiblyInfiniteTreeWithRoot
+section ChildTrees
 
-    def opt_to_tree (opt : Option (PossiblyInfiniteTreeWithRoot α)) : PossiblyInfiniteTree α :=
-      match opt with
-      | .none => PossiblyInfiniteTree.empty
-      | .some t => t.val
+/-!
+## Child Trees
 
-    theorem opt_to_tree_none_iff {opt : Option (PossiblyInfiniteTreeWithRoot α)} : opt = none ↔ (opt_to_tree opt).root = none := by
-      unfold opt_to_tree
-      cases opt with
-      | none => simp [root_empty]
-      | some t => simp [t.property]
+Defining the `childTrees` function requires a bit of machinery.
+We only want to return the child trees that are not already empty.
+Then all returned trees have a non-none root, which we aim to capture directly in the return type.
+-/
 
-    def tree_to_opt (t : PossiblyInfiniteTree α) : Option (PossiblyInfiniteTreeWithRoot α) :=
-      match eq : t.root with
-      | .none => none
-      | .some r => some ⟨t, by simp [eq]⟩
+/-- The `PossiblyInfiniteTreeWithRoot` is a `PossiblyInfiniteTree` where the `root` is not none. -/
+abbrev PossiblyInfiniteTreeWithRoot (α : Type u) := {t : PossiblyInfiniteTree α // t.root ≠ none}
 
-    theorem tree_to_opt_none_iff {t : PossiblyInfiniteTree α} : tree_to_opt t = none ↔ t.root = none := by
-      unfold tree_to_opt
-      split; simpa; simp [*]
+namespace PossiblyInfiniteTreeWithRoot
 
-    theorem tree_to_opt_some_iff {t : PossiblyInfiniteTree α} : ∀ {t'}, tree_to_opt t = some t' ↔ t = t' ∧ t.root.isSome := by
-      unfold tree_to_opt
-      split
-      case h_1 eq => simp [eq]
-      case h_2 eq => simp [eq]
+/-!
+### PossiblyInfiniteTreeWithRoot
 
-    theorem tree_to_opt_after_opt_to_tree {opt : Option (PossiblyInfiniteTreeWithRoot α)} :
-        tree_to_opt (opt_to_tree opt) = opt := by
-      cases eq : opt with
-      | none => rw [tree_to_opt_none_iff, ← opt_to_tree_none_iff]
-      | some t =>
-        simp only [opt_to_tree, tree_to_opt]
-        split
-        . have := t.property; contradiction
-        . rfl
+For the `PossiblyInfiniteTreeWithRoot` we mainly provide some functions to convert `PossiblyInfiniteTree` to and from `Option PossiblyInfiniteTreeWithRoot`. Clearly, if a `PossiblyInfiniteTree` has a non-none root, we can convert it directly into a `PossiblyInfiniteTreeWithRoot`, otherwise, we simply convert it to `none`. Also in the other direction, none can just be converted to `PossiblyInfiniteTree.empty` and any `PossiblyInfiniteTreeWithRoot` is already a `PossiblyInfiniteTree`.
+-/
 
-    theorem opt_to_tree_after_tree_to_opt {t : PossiblyInfiniteTree α} :
-        opt_to_tree (tree_to_opt t) = t := by
-      unfold tree_to_opt
-      split
-      . simp only [opt_to_tree]; apply Eq.symm; rw [empty_iff_root_none]; assumption
-      . simp only [opt_to_tree]
+def opt_to_tree (opt : Option (PossiblyInfiniteTreeWithRoot α)) : PossiblyInfiniteTree α :=
+  match opt with
+  | .none => PossiblyInfiniteTree.empty
+  | .some t => t.val
 
-  end PossiblyInfiniteTreeWithRoot
+def tree_to_opt (t : PossiblyInfiniteTree α) : Option (PossiblyInfiniteTreeWithRoot α) :=
+  match eq : t.root with
+  | .none => none
+  | .some r => some ⟨t, by simp [eq]⟩
 
-  def childTrees (t : PossiblyInfiniteTree α) : PossiblyInfiniteList (PossiblyInfiniteTreeWithRoot α) where
-    infinite_list := fun n => PossiblyInfiniteTreeWithRoot.tree_to_opt {
-      infinite_tree := t.infinite_tree.childTrees.get n
-      no_orphans := by intro ns; rw [InfiniteTreeSkeleton.get_get_childTrees]; intro eq_none n'; rw [InfiniteTreeSkeleton.get_childTrees, InfiniteTreeSkeleton.drop_drop]; apply t.no_orphans; exact eq_none
-      no_holes_in_children := by intro _ suf; apply t.no_holes_in_children; exact InfiniteTreeSkeleton.IsSuffix_trans suf (t.infinite_tree.IsSuffix_of_mem_childTrees _ InfiniteList.get_mem)
-    }
-    no_holes := by intro n'; simp only [InfiniteList.get]; rw [PossiblyInfiniteTreeWithRoot.tree_to_opt_none_iff, PossiblyInfiniteTreeWithRoot.tree_to_opt_none_iff]; exact t.no_holes_in_children _ InfiniteTreeSkeleton.IsSuffix_refl n'
+theorem opt_to_tree_none_iff {opt : Option (PossiblyInfiniteTreeWithRoot α)} : opt = none ↔ (opt_to_tree opt).root = none := by
+  unfold opt_to_tree
+  cases opt with
+  | none => simp [root_empty]
+  | some t => simp [t.property]
 
-  theorem mem_childTrees_iff {t : PossiblyInfiniteTree α} : ∀ c, c ∈ t.childTrees ↔ c.val.infinite_tree ∈ t.infinite_tree.childTrees := by
-    intro c; unfold childTrees
-    simp only [PossiblyInfiniteList.mem_iff, PossiblyInfiniteList.get?, InfiniteList.get, PossiblyInfiniteTreeWithRoot.tree_to_opt_some_iff]
-    constructor
-    . rintro ⟨n, mem⟩
-      exists n
-      rw [← mem.left]
-      rfl
-    . rintro ⟨n, mem⟩
-      simp only [InfiniteList.get] at mem
-      exists n
-      constructor
-      . rw [PossiblyInfiniteTree.mk.injEq]; exact mem
-      . simp only [root]
-        rw [mem, Option.isSome_iff_ne_none]
-        exact c.property
+theorem tree_to_opt_none_iff {t : PossiblyInfiniteTree α} : tree_to_opt t = none ↔ t.root = none := by
+  unfold tree_to_opt
+  split; simpa; simp [*]
 
-  theorem childTrees_empty {α} : (@PossiblyInfiniteTree.empty α).childTrees = PossiblyInfiniteList.empty := by rfl
+theorem tree_to_opt_some_iff {t : PossiblyInfiniteTree α} : ∀ {t'}, tree_to_opt t = some t' ↔ t = t' ∧ t.root.isSome := by
+  unfold tree_to_opt
+  split
+  case h_1 eq => simp [eq]
+  case h_2 eq => simp [eq]
 
-  theorem IsSuffix_of_mem_childTrees {t : PossiblyInfiniteTree α} : ∀ c ∈ t.childTrees, c <:+ t := by
-    intro c c_mem; apply t.infinite_tree.IsSuffix_of_mem_childTrees; rw [mem_childTrees_iff] at c_mem; exact c_mem
+theorem tree_to_opt_after_opt_to_tree {opt : Option (PossiblyInfiniteTreeWithRoot α)} :
+    tree_to_opt (opt_to_tree opt) = opt := by
+  cases eq : opt with
+  | none => rw [tree_to_opt_none_iff, ← opt_to_tree_none_iff]
+  | some t =>
+    simp only [opt_to_tree, tree_to_opt]
+    split
+    . have := t.property; contradiction
+    . rfl
 
-  def node (root : α) (childTrees : PossiblyInfiniteList (PossiblyInfiniteTreeWithRoot α)) : PossiblyInfiniteTree α where
-    infinite_tree := InfiniteTreeSkeleton.node (.some root) (childTrees.infinite_list.map (PossiblyInfiniteTree.infinite_tree ∘ PossiblyInfiniteTreeWithRoot.opt_to_tree))
-    no_orphans := by
-      intro ns
-      cases ns with
-      | nil => intro contra; rw [← InfiniteTreeSkeleton.root.eq_def, InfiniteTreeSkeleton.root_node] at contra; simp at contra
-      | cons n ns =>
-        rw [← InfiniteTreeSkeleton.childTrees.eq_def, InfiniteTreeSkeleton.childTrees_node]
-        intro eq_none n'
-        unfold InfiniteList.map at eq_none
-        rw [InfiniteTreeSkeleton.drop_node_cons, InfiniteList.get_map]
-        apply (PossiblyInfiniteTreeWithRoot.opt_to_tree (childTrees.infinite_list.get n)).no_orphans
-        exact eq_none
-    no_holes_in_children := by
-      rintro _ ⟨ns, eq⟩
-      cases ns with
-      | nil => rw [← eq, InfiniteTreeSkeleton.drop_nil]; unfold InfiniteTreeSkeleton.childNodes; rw [InfiniteTreeSkeleton.childTrees_node]; intro n; simp only [InfiniteList.get_map, Function.comp_apply]; rw [← PossiblyInfiniteTree.root.eq_def, ← PossiblyInfiniteTree.root.eq_def, ← PossiblyInfiniteTreeWithRoot.opt_to_tree_none_iff, ← PossiblyInfiniteTreeWithRoot.opt_to_tree_none_iff]; exact childTrees.no_holes n
-      | cons n ns =>
-        rw [← eq, InfiniteTreeSkeleton.drop_node_cons, InfiniteList.get_map]
-        exact (PossiblyInfiniteTreeWithRoot.opt_to_tree (childTrees.infinite_list.get n)).no_holes_in_children _ (by exists ns)
+theorem opt_to_tree_after_tree_to_opt {t : PossiblyInfiniteTree α} :
+    opt_to_tree (tree_to_opt t) = t := by
+  unfold tree_to_opt
+  split
+  . simp only [opt_to_tree]; apply Eq.symm; rw [empty_iff_root_none]; assumption
+  . simp only [opt_to_tree]
 
-  theorem get?_node_nil {root : α} {childTrees : PossiblyInfiniteList (PossiblyInfiniteTreeWithRoot α)} : (node root childTrees).get? [] = .some root := by rfl
-  theorem get?_node_cons {root : α} {childTrees : PossiblyInfiniteList (PossiblyInfiniteTreeWithRoot α)} : ∀ n ns, (node root childTrees).get? (n :: ns) = (PossiblyInfiniteTreeWithRoot.opt_to_tree (childTrees.get? n)).get? ns := by intro n ns; rfl
+end PossiblyInfiniteTreeWithRoot
 
-  theorem root_node {root : α} {childTrees : PossiblyInfiniteList (PossiblyInfiniteTreeWithRoot α)} : (node root childTrees).root = root := by rfl
-  theorem childTrees_node {root : α} {childTrees : PossiblyInfiniteList (PossiblyInfiniteTreeWithRoot α)} : (node root childTrees).childTrees = childTrees := by
-    unfold node PossiblyInfiniteTree.childTrees
-    simp only [InfiniteTreeSkeleton.childTrees_node, InfiniteList.get_map, Function.comp_apply]
-    apply PossiblyInfiniteList.ext
-    intro n
-    simp only [PossiblyInfiniteList.get?, InfiniteList.get]
-    rw [PossiblyInfiniteTreeWithRoot.tree_to_opt_after_opt_to_tree]
+/-!
+### The actual childTrees definition
 
-  theorem node_root_childTrees {t : PossiblyInfiniteTree α} {root : α} (h : t.root = .some root) : t = node root t.childTrees := by
-    rw [PossiblyInfiniteTree.mk.injEq]; simp only [node]; rw [← h]; rw [InfiniteTreeSkeleton.node_root_childTrees t.infinite_tree]
-    apply congrArg
-    unfold PossiblyInfiniteTree.childTrees
-    apply InfiniteList.ext
-    intro n
-    simp only [InfiniteList.get_map, Function.comp_apply]
-    simp only [InfiniteList.get]
-    rw [PossiblyInfiniteTreeWithRoot.opt_to_tree_after_tree_to_opt]
+With `PossiblyInfiniteTreeWithRoot` in place, we can now define the actual `childTrees` function.
+-/
 
-  theorem get?_childTrees {t : PossiblyInfiniteTree α} : ∀ n, (t.childTrees.get? n) = PossiblyInfiniteTreeWithRoot.tree_to_opt (t.drop [n]) := by intros; rfl
-  theorem get?_get?_childTrees {t : PossiblyInfiniteTree α} : ∀ n ns, (PossiblyInfiniteTreeWithRoot.opt_to_tree (t.childTrees.get? n)).get? ns = t.get? (n::ns) := by intros; rw [get?_childTrees, PossiblyInfiniteTreeWithRoot.opt_to_tree_after_tree_to_opt]; rfl
+/-- The `childTrees` of a `PossiblyInfiniteTree` are the `PossiblyInfiniteList` of all child trees that are not empty, i.e. it only consists of `PossiblyInfiniteTreeWithRoot`. -/
+def childTrees (t : PossiblyInfiniteTree α) : PossiblyInfiniteList (PossiblyInfiniteTreeWithRoot α) where
+  infinite_list := fun n => PossiblyInfiniteTreeWithRoot.tree_to_opt {
+    infinite_tree := t.infinite_tree.childTrees.get n
+    no_orphans := by intro ns; rw [InfiniteTreeSkeleton.get_get_childTrees]; intro eq_none n'; rw [InfiniteTreeSkeleton.get_childTrees, InfiniteTreeSkeleton.drop_drop]; apply t.no_orphans; exact eq_none
+    no_holes_in_children := by intro _ suf; apply t.no_holes_in_children; exact InfiniteTreeSkeleton.IsSuffix_trans suf (t.infinite_tree.IsSuffix_of_mem_childTrees _ InfiniteList.get_mem)
+  }
+  no_holes := by intro n'; simp only [InfiniteList.get]; rw [PossiblyInfiniteTreeWithRoot.tree_to_opt_none_iff, PossiblyInfiniteTreeWithRoot.tree_to_opt_none_iff]; exact t.no_holes_in_children _ InfiniteTreeSkeleton.IsSuffix_refl n'
 
-  theorem drop_node_cons {root : α} {childTrees : PossiblyInfiniteList (PossiblyInfiniteTreeWithRoot α)} {n : Nat} {ns : List Nat} : (node root childTrees).drop (n::ns) = (PossiblyInfiniteTreeWithRoot.opt_to_tree (childTrees.get? n)).drop ns := by rfl
-
-  def childNodes (t : PossiblyInfiniteTree α) : PossiblyInfiniteList α where
-    infinite_list := t.infinite_tree.childNodes
-    no_holes := t.no_holes_in_children _ InfiniteTreeSkeleton.IsSuffix_refl
-
-  theorem get?_childNodes {t : PossiblyInfiniteTree α} : ∀ {n}, t.childNodes.get? n = (PossiblyInfiniteTreeWithRoot.opt_to_tree (t.childTrees.get? n)).root := by
-    intro n; rw [get?_childTrees, PossiblyInfiniteTreeWithRoot.opt_to_tree_after_tree_to_opt]; rfl
-
-  theorem childNodes_eq {t : PossiblyInfiniteTree α} : t.childNodes = t.childTrees.map (fun t => t.val.root.get (by rw [Option.isSome_iff_ne_none]; exact t.property)) := by
-    apply PossiblyInfiniteList.ext
-    intro n
-    rw [PossiblyInfiniteList.get?_map]
-    rw [get?_childNodes, get?_childTrees, PossiblyInfiniteTreeWithRoot.opt_to_tree_after_tree_to_opt]
-    apply Eq.symm
-    cases eq : (t.drop [n]).root with
-    | none => rw [Option.map_eq_none_iff, PossiblyInfiniteTreeWithRoot.tree_to_opt_none_iff]; exact eq
-    | some r => rw [Option.map_eq_some_iff]; exists ⟨t.drop [n], by simp [eq]⟩; rw [PossiblyInfiniteTreeWithRoot.tree_to_opt_some_iff]; simp [eq]
-
-  theorem childNodes_empty {α} : (@PossiblyInfiniteTree.empty α).childNodes = PossiblyInfiniteList.empty := by
-    apply PossiblyInfiniteList.ext; intro _; rw [get?_childNodes, childTrees_empty, PossiblyInfiniteList.get?_empty, PossiblyInfiniteList.get?_empty, ← PossiblyInfiniteTreeWithRoot.opt_to_tree_none_iff]
-
-  theorem mem_of_mem_childNodes {t : PossiblyInfiniteTree α} : ∀ c ∈ t.childNodes, c ∈ t := by
-    intro c; exact t.infinite_tree.mem_of_mem_childNodes (some c)
-
-  theorem mem_rec
-      {t : PossiblyInfiniteTree α}
-      {motive : Element t -> Prop}
-      (root : ∀ r, (mem : r ∈ t.root) -> motive ⟨r, root_mem _ mem⟩)
-      (step : ∀ t2, (suffix : t2 <:+ t) -> (∃ (r : α) (mem : r ∈ t2.root), motive ⟨r, t2.mem_of_mem_suffix suffix _ (t2.root_mem _ mem)⟩) -> ∀ {c}, (mem : c ∈ t2.childNodes) -> motive ⟨c, mem_of_mem_suffix suffix _ (mem_of_mem_childNodes _ mem)⟩)
-      (a : Element t) :
-      motive a := by
-    let motive' (o : t.infinite_tree.Element) : Prop := ∀ v, (mem : v ∈ o.val) -> motive ⟨v, by have := o.property; rw [Option.mem_def] at mem; rw [mem] at this; exact this⟩
-    let a' : t.infinite_tree.Element := ⟨some a.val, a.property⟩
-    have : motive' a' := by
-      induction a' using InfiniteTreeSkeleton.mem_rec with
-      | root => exact root
-      | step t2 suffix ih c_mem =>
-        rcases suffix with ⟨ns, suffix⟩
-        rcases c_mem with ⟨m, c_mem⟩
-        rw [← suffix] at c_mem
-        simp only [← c_mem]
-        cases eq : (t.infinite_tree.drop ns).root with
-        | none =>
-          intro _ mem
-          rw [InfiniteTreeSkeleton.root_drop] at eq
-          simp [(t.no_orphans ns eq m)] at mem
-        | some r =>
-          specialize step (t.drop ns) (t.IsSuffix_drop ns)
-          intro v v_mem
-          apply step
-          . exists r, eq; apply ih; simp [← suffix, eq]
-          . exists m
-    apply this
+/-- `PossiblyInfiniteTree.childTrees` can be expressed through `InfiniteList.childTrees`. -/
+theorem mem_childTrees_iff {t : PossiblyInfiniteTree α} : ∀ c, c ∈ t.childTrees ↔ c.val.infinite_tree ∈ t.infinite_tree.childTrees := by
+  intro c; unfold childTrees
+  simp only [PossiblyInfiniteList.mem_iff, PossiblyInfiniteList.get?, InfiniteList.get, PossiblyInfiniteTreeWithRoot.tree_to_opt_some_iff]
+  constructor
+  . rintro ⟨n, mem⟩
+    exists n
+    rw [← mem.left]
     rfl
-
-  theorem no_orphans' {t : PossiblyInfiniteTree α} : ∀ ns : List Nat, t.get? ns = none -> ∀ n, (t.drop ns).childNodes.get? n = none := by exact t.no_orphans
-
-  theorem no_orphans'_closure {t : PossiblyInfiniteTree α} :
-      ∀ ns : List Nat, t.get? ns = none -> ∀ ns', (t.drop ns).get? ns' = none := by
-    exact t.infinite_tree.no_orphans_closure t.no_orphans
-
-  def branchForAddress (t : PossiblyInfiniteTree α) (ns : InfiniteList Nat) : PossiblyInfiniteList α where
-    infinite_list := t.infinite_tree.branchForAddress ns
-    no_holes := by
-      intro n
-      rw [InfiniteTreeSkeleton.get_branchForAddress]
-      intro eq_none
-      rw [InfiniteTreeSkeleton.get_branchForAddress]
-      rw [InfiniteList.take_succ']
-      apply t.no_orphans
-      exact eq_none
-
-  theorem get?_branchForAddress {t : PossiblyInfiniteTree α} {ns : InfiniteList Nat} {n : Nat} : (t.branchForAddress ns).get? n = t.get? (ns.take n) := by rfl
-
-  def branchAddressIsMaximal (t : PossiblyInfiniteTree α) (ns : InfiniteList Nat) : Prop :=
-    ∀ n, (t.branchForAddress ns).get? n.succ = none -> (t.drop (ns.take n)).childNodes.head = none
-
-  def branches (t : PossiblyInfiniteTree α) : Set (PossiblyInfiniteList α) :=
-    fun b => ∃ ns, b = t.branchForAddress ns ∧ t.branchAddressIsMaximal ns
-
-  theorem branches_eq {t : PossiblyInfiniteTree α} : t.branches = fun b =>
-      b.head = t.root ∧ ((t.childTrees = PossiblyInfiniteList.empty ∧ b.tail = PossiblyInfiniteList.empty) ∨ (∃ c ∈ t.childTrees, b.tail ∈ c.val.branches)) := by
-    unfold branches
-    apply Set.ext
-    intro b
+  . rintro ⟨n, mem⟩
+    simp only [InfiniteList.get] at mem
+    exists n
     constructor
-    . rintro ⟨ns, b_eq, ns_max⟩
-      constructor
-      . rw [b_eq]; rfl
-      . cases eq : t.childTrees.get? (ns.get 0) with
-        | none =>
-          apply Or.inl
-          rw [get?_childTrees] at eq
-          rw [PossiblyInfiniteTreeWithRoot.tree_to_opt_none_iff] at eq
-          rw [root_drop] at eq
-          rw [PossiblyInfiniteList.empty_iff_head_none]
-          rw [PossiblyInfiniteList.empty_iff_head_none]
-          constructor
-          . specialize ns_max 0
-            rw [get?_branchForAddress] at ns_max
-            rw [InfiniteList.take_succ, InfiniteList.take_zero, InfiniteList.take_zero, drop_nil] at ns_max
-            unfold InfiniteList.head at ns_max
-            specialize ns_max eq
-            rw [PossiblyInfiniteList.head_eq] at ns_max
-            rw [PossiblyInfiniteList.head_eq]
-            rw [get?_childNodes, ← PossiblyInfiniteTreeWithRoot.opt_to_tree_none_iff] at ns_max
-            exact ns_max
-          . rw [b_eq]
-            rw [PossiblyInfiniteList.head_eq, PossiblyInfiniteList.get?_tail]
-            rw [get?_branchForAddress]
-            rw [InfiniteList.take_succ, InfiniteList.take_zero]
-            unfold InfiniteList.head
-            exact eq
-        | some c =>
-          apply Or.inr
-          exists c
-          constructor
-          . exists ns.get 0
-          exists ns.tail
-          rw [get?_childTrees] at eq
-          rw [PossiblyInfiniteTreeWithRoot.tree_to_opt_some_iff] at eq
-          constructor
-          . rw [b_eq]
-            apply PossiblyInfiniteList.ext
-            intro n
-            rw [PossiblyInfiniteList.get?_tail]
-            rw [get?_branchForAddress]
-            rw [get?_branchForAddress]
-            rw [InfiniteList.take_succ]
-            rw [← List.singleton_append]
-            rw [← get?_drop]
-            unfold InfiniteList.head
-            rw [eq.left]
-          . intro n
-            specialize ns_max (n+1)
-            rw [get?_branchForAddress] at ns_max
-            rw [InfiniteList.take_succ] at ns_max
-            rw [← List.singleton_append] at ns_max
-            rw [← get?_drop] at ns_max
-            unfold InfiniteList.head at ns_max
-            rw [eq.left] at ns_max
-            rw [get?_branchForAddress]
-            intro h
-            specialize ns_max h
-            rw [InfiniteList.take_succ] at ns_max
-            rw [← List.singleton_append] at ns_max
-            rw [← drop_drop] at ns_max
-            unfold InfiniteList.head at ns_max
-            rw [eq.left] at ns_max
-            exact ns_max
-    . rintro ⟨head_eq, tail_eq⟩
-      cases tail_eq with
-      | inl tail_eq =>
-        exists fun _ => 0
+    . rw [PossiblyInfiniteTree.mk.injEq]; exact mem
+    . simp only [root]
+      rw [mem, Option.isSome_iff_ne_none]
+      exact c.property
+
+/-- Getting a child tree is the same as dropping the corresponding singleton address. -/
+theorem get?_childTrees {t : PossiblyInfiniteTree α} : ∀ n, (t.childTrees.get? n) = PossiblyInfiniteTreeWithRoot.tree_to_opt (t.drop [n]) := by intros; rfl
+
+/-- Getting at an address in a child tree can be combined into a single get call. -/
+theorem get?_get?_childTrees {t : PossiblyInfiniteTree α} : ∀ n ns, (PossiblyInfiniteTreeWithRoot.opt_to_tree (t.childTrees.get? n)).get? ns = t.get? (n::ns) := by intros; rw [get?_childTrees, PossiblyInfiniteTreeWithRoot.opt_to_tree_after_tree_to_opt]; rfl
+
+/-- The `childTrees` of the `empty` tree are exactly `PossiblyInfiniteList.empty`. -/
+theorem childTrees_empty {α} : (@PossiblyInfiniteTree.empty α).childTrees = PossiblyInfiniteList.empty := by rfl
+
+end ChildTrees
+
+section Node
+
+/-!
+## Node Constructor
+
+Similar to the `InfiniteTreeSkeleton`, we can also define a `node` constructor on the `PossiblyInfiniteTree`.
+-/
+
+/-- Construct a `PossiblyInfiniteTree` from a `PossiblyInfiniteList` of `PossiblyInfiniteTreeWithRoot` and a new root element. -/
+def node (root : α) (childTrees : PossiblyInfiniteList (PossiblyInfiniteTreeWithRoot α)) : PossiblyInfiniteTree α where
+  infinite_tree := InfiniteTreeSkeleton.node (.some root) (childTrees.infinite_list.map (PossiblyInfiniteTree.infinite_tree ∘ PossiblyInfiniteTreeWithRoot.opt_to_tree))
+  no_orphans := by
+    intro ns
+    cases ns with
+    | nil => intro contra; rw [← InfiniteTreeSkeleton.root.eq_def, InfiniteTreeSkeleton.root_node] at contra; simp at contra
+    | cons n ns =>
+      rw [← InfiniteTreeSkeleton.childTrees.eq_def, InfiniteTreeSkeleton.childTrees_node]
+      intro eq_none n'
+      unfold InfiniteList.map at eq_none
+      rw [InfiniteTreeSkeleton.drop_node_cons, InfiniteList.get_map]
+      apply (PossiblyInfiniteTreeWithRoot.opt_to_tree (childTrees.infinite_list.get n)).no_orphans
+      exact eq_none
+  no_holes_in_children := by
+    rintro _ ⟨ns, eq⟩
+    cases ns with
+    | nil => rw [← eq, InfiniteTreeSkeleton.drop_nil]; unfold InfiniteTreeSkeleton.childNodes; rw [InfiniteTreeSkeleton.childTrees_node]; intro n; simp only [InfiniteList.get_map, Function.comp_apply]; rw [← PossiblyInfiniteTree.root.eq_def, ← PossiblyInfiniteTree.root.eq_def, ← PossiblyInfiniteTreeWithRoot.opt_to_tree_none_iff, ← PossiblyInfiniteTreeWithRoot.opt_to_tree_none_iff]; exact childTrees.no_holes n
+    | cons n ns =>
+      rw [← eq, InfiniteTreeSkeleton.drop_node_cons, InfiniteList.get_map]
+      exact (PossiblyInfiniteTreeWithRoot.opt_to_tree (childTrees.infinite_list.get n)).no_holes_in_children _ (by exists ns)
+
+/-- Getting the element at address [] on `node` is the new root. -/
+theorem get?_node_nil {root : α} {childTrees : PossiblyInfiniteList (PossiblyInfiniteTreeWithRoot α)} : (node root childTrees).get? [] = .some root := by rfl
+
+/-- Getting any address != [] on `node` yields the respective element from the previous `PossiblyInfiniteTreeWithRoot`. -/
+theorem get?_node_cons {root : α} {childTrees : PossiblyInfiniteList (PossiblyInfiniteTreeWithRoot α)} : ∀ n ns, (node root childTrees).get? (n :: ns) = (PossiblyInfiniteTreeWithRoot.opt_to_tree (childTrees.get? n)).get? ns := by intro n ns; rfl
+
+/-- Dropping from `node` with an address of the form `n::ns` is the same as getting the `n` child from the child trees used in the construction and then dropping `ns` there.  -/
+theorem drop_node_cons {root : α} {childTrees : PossiblyInfiniteList (PossiblyInfiniteTreeWithRoot α)} {n : Nat} {ns : List Nat} : (node root childTrees).drop (n::ns) = (PossiblyInfiniteTreeWithRoot.opt_to_tree (childTrees.get? n)).drop ns := by rfl
+
+/-- The `root` of `node` is the root used in the construction. -/
+theorem root_node {root : α} {childTrees : PossiblyInfiniteList (PossiblyInfiniteTreeWithRoot α)} : (node root childTrees).root = root := by rfl
+
+/-- The `childTrees` of `node` are the childTrees used in the construction. -/
+theorem childTrees_node {root : α} {childTrees : PossiblyInfiniteList (PossiblyInfiniteTreeWithRoot α)} : (node root childTrees).childTrees = childTrees := by
+  unfold node PossiblyInfiniteTree.childTrees
+  simp only [InfiniteTreeSkeleton.childTrees_node, InfiniteList.get_map, Function.comp_apply]
+  apply PossiblyInfiniteList.ext
+  intro n
+  simp only [PossiblyInfiniteList.get?, InfiniteList.get]
+  rw [PossiblyInfiniteTreeWithRoot.tree_to_opt_after_opt_to_tree]
+
+/-- Any `PossiblyInfiniteTree` where the `root` is not none can be written using the `node` constructor. -/
+theorem node_root_childTrees {t : PossiblyInfiniteTree α} {root : α} (h : t.root = .some root) : t = node root t.childTrees := by
+  rw [PossiblyInfiniteTree.mk.injEq]; simp only [node]; rw [← h]; rw [InfiniteTreeSkeleton.node_root_childTrees t.infinite_tree]
+  apply congrArg
+  unfold PossiblyInfiniteTree.childTrees
+  apply InfiniteList.ext
+  intro n
+  simp only [InfiniteList.get_map, Function.comp_apply]
+  simp only [InfiniteList.get]
+  rw [PossiblyInfiniteTreeWithRoot.opt_to_tree_after_tree_to_opt]
+
+end Node
+
+section ChildNodes
+
+/-!
+# ChildNodes
+
+It can be convenient to obtain a list of the immediate child nodes of a given tree.
+This is equivalent to mapping each child tree to its root.
+-/
+
+/-- The `childNodes` are `InfiniteTreeSkeleton.childNodes`. -/
+def childNodes (t : PossiblyInfiniteTree α) : PossiblyInfiniteList α where
+  infinite_list := t.infinite_tree.childNodes
+  no_holes := t.no_holes_in_children _ InfiniteTreeSkeleton.IsSuffix_refl
+
+/-- Getting the nth `childNodes` is the root of the nth `childTrees`. -/
+theorem get?_childNodes {t : PossiblyInfiniteTree α} : ∀ {n}, t.childNodes.get? n = (PossiblyInfiniteTreeWithRoot.opt_to_tree (t.childTrees.get? n)).root := by
+  intro n; rw [get?_childTrees, PossiblyInfiniteTreeWithRoot.opt_to_tree_after_tree_to_opt]; rfl
+
+/-- The `childNodes` are the `root`s of the `childTrees`. -/
+theorem childNodes_eq {t : PossiblyInfiniteTree α} : t.childNodes = t.childTrees.map (fun t => t.val.root.get (by rw [Option.isSome_iff_ne_none]; exact t.property)) := by
+  apply PossiblyInfiniteList.ext
+  intro n
+  rw [PossiblyInfiniteList.get?_map]
+  rw [get?_childNodes, get?_childTrees, PossiblyInfiniteTreeWithRoot.opt_to_tree_after_tree_to_opt]
+  apply Eq.symm
+  cases eq : (t.drop [n]).root with
+  | none => rw [Option.map_eq_none_iff, PossiblyInfiniteTreeWithRoot.tree_to_opt_none_iff]; exact eq
+  | some r => rw [Option.map_eq_some_iff]; exists ⟨t.drop [n], by simp [eq]⟩; rw [PossiblyInfiniteTreeWithRoot.tree_to_opt_some_iff]; simp [eq]
+
+/-- Each child node is a tree member. -/
+theorem mem_of_mem_childNodes {t : PossiblyInfiniteTree α} : ∀ c ∈ t.childNodes, c ∈ t := by
+  intro c; exact t.infinite_tree.mem_of_mem_childNodes (some c)
+
+/-- The `childNodes` of the `empty` tree are `PossiblyInfiniteList.empty`. -/
+theorem childNodes_empty {α} : (@PossiblyInfiniteTree.empty α).childNodes = PossiblyInfiniteList.empty := by
+  apply PossiblyInfiniteList.ext; intro _; rw [get?_childNodes, childTrees_empty, PossiblyInfiniteList.get?_empty, PossiblyInfiniteList.get?_empty, ← PossiblyInfiniteTreeWithRoot.opt_to_tree_none_iff]
+
+/-- We can express the `InfiniteTreeSkeleton.no_orphans` condition directly on `PossiblyInfiniteTree`. -/
+theorem no_orphans' {t : PossiblyInfiniteTree α} : ∀ ns : List Nat, t.get? ns = none -> ∀ n, (t.drop ns).childNodes.get? n = none := by exact t.no_orphans
+
+/-- We can also express the `InfiniteTreeSkeleton.no_orphans_closure` directly on `PossiblyInfiniteTree`. -/
+theorem no_orphans'_closure {t : PossiblyInfiniteTree α} :
+    ∀ ns : List Nat, t.get? ns = none -> ∀ ns', (t.drop ns).get? ns' = none := by
+  exact t.infinite_tree.no_orphans_closure t.no_orphans
+
+end ChildNodes
+
+section Suffixes
+
+/-!
+## Suffixes
+
+Here, we define a suffix relation on `PossiblyInfiniteTree` inspired by `List.IsSuffix`.
+For `t1` and `t2`, `t1 <:+ t2` denotes that `t1` is a subtree of `t2`.
+
+The suffix relation is reflexive and transitive but not necesarrily antisymmetric!
+Note also that `InfiniteList.suffix_or_suffix_of_suffix` has no equivalent statement here, i.e.
+just because two trees are subtrees of the same parent tree, we cannot say anything about their relation to one another.
+They might be totally "disconnected".
+-/
+
+/-- A suffix relation on infinite trees. This is inspired by `List.IsSuffix`. Read `t1 <:+ t2` as: t1 is a subtree of t2. -/
+def IsSuffix (t1 t2 : PossiblyInfiniteTree α) : Prop := t1.infinite_tree <:+ t2.infinite_tree
+infixl:50 " <:+ " => IsSuffix
+
+/-- t1 is a subtree of t2 if t1 can be obtained from t2 by dropping. -/
+theorem IsSuffix_iff {t1 t2 : PossiblyInfiniteTree α} : t1 <:+ t2 ↔ ∃ ns, t2.drop ns = t1 := by
+  constructor
+  . rintro ⟨ns, h⟩; exists ns; simp [drop, h]
+  . rintro ⟨ns, h⟩; exists ns; simp only [drop] at h; rw [← h]
+
+/-- The suffix relation is reflexive. -/
+theorem IsSuffix_refl {t : PossiblyInfiniteTree α} : t <:+ t := t.infinite_tree.IsSuffix_refl
+
+/-- The suffix relation is transitive. -/
+theorem IsSuffix_trans {t1 t2 t3 : PossiblyInfiniteTree α} : t1 <:+ t2 -> t2 <:+ t3 -> t1 <:+ t3 := InfiniteTreeSkeleton.IsSuffix_trans
+
+/-- A member of a subtree is also a member of the current tree. -/
+theorem mem_of_mem_suffix {t1 t2 : PossiblyInfiniteTree α} (suffix : t1 <:+ t2) : ∀ e ∈ t1, e ∈ t2 := by
+  intro e mem; apply InfiniteTreeSkeleton.mem_of_mem_suffix suffix; exact mem
+
+/-- Dropping elements yields a subtree. -/
+theorem IsSuffix_drop {t : PossiblyInfiniteTree α} : ∀ ns, t.drop ns <:+ t := t.infinite_tree.IsSuffix_drop
+
+/-- Each child tree is a subtree. -/
+theorem IsSuffix_of_mem_childTrees {t : PossiblyInfiniteTree α} : ∀ c ∈ t.childTrees, c <:+ t := by
+  intro c c_mem; apply t.infinite_tree.IsSuffix_of_mem_childTrees; rw [mem_childTrees_iff] at c_mem; exact c_mem
+
+end Suffixes
+
+section ElementRecursor
+
+/-!
+## Recursor for Members
+
+We define a recursion (induction) principle for members (`Element`s) of an `PossiblyInfiniteTree` called `mem_rec`.
+This can be used with the `induction` tactic to prove a property for each `Element` of an `PossiblyInfiniteTree`.
+Note that for using this coveniently, the goal needs to expressed (rewritten) using an `Element`.
+-/
+
+/-- A tree `Element` is a Subtype featuring a proof of being a tree member. -/
+def Element (t : PossiblyInfiniteTree α) := { e : α // e ∈ t }
+
+/-- A recursor for proving properties about tree members (`Element`s) via induction. -/
+theorem mem_rec
+    {t : PossiblyInfiniteTree α}
+    {motive : Element t -> Prop}
+    (root : ∀ r, (mem : r ∈ t.root) -> motive ⟨r, root_mem _ mem⟩)
+    (step : ∀ t2, (suffix : t2 <:+ t) -> (∃ (r : α) (mem : r ∈ t2.root), motive ⟨r, t2.mem_of_mem_suffix suffix _ (t2.root_mem _ mem)⟩) -> ∀ {c}, (mem : c ∈ t2.childNodes) -> motive ⟨c, mem_of_mem_suffix suffix _ (mem_of_mem_childNodes _ mem)⟩)
+    (a : Element t) :
+    motive a := by
+  let motive' (o : t.infinite_tree.Element) : Prop := ∀ v, (mem : v ∈ o.val) -> motive ⟨v, by have := o.property; rw [Option.mem_def] at mem; rw [mem] at this; exact this⟩
+  let a' : t.infinite_tree.Element := ⟨some a.val, a.property⟩
+  have : motive' a' := by
+    induction a' using InfiniteTreeSkeleton.mem_rec with
+    | root => exact root
+    | step t2 suffix ih c_mem =>
+      rcases suffix with ⟨ns, suffix⟩
+      rcases c_mem with ⟨m, c_mem⟩
+      rw [← suffix] at c_mem
+      simp only [← c_mem]
+      cases eq : (t.infinite_tree.drop ns).root with
+      | none =>
+        intro _ mem
+        rw [InfiniteTreeSkeleton.root_drop] at eq
+        simp [(t.no_orphans ns eq m)] at mem
+      | some r =>
+        specialize step (t.drop ns) (t.IsSuffix_drop ns)
+        intro v v_mem
+        apply step
+        . exists r, eq; apply ih; simp [← suffix, eq]
+        . exists m
+  apply this
+  rfl
+
+end ElementRecursor
+
+section Branches
+
+/-!
+# Branches
+
+Branches are essentially `PossiblyInfiniteList`s in an `PossiblyInfiniteTree`
+and can be characterizes by an infinite "address", i.e. `InfiniteList Nat`.
+-/
+
+/-- This function defines the `PossiblyInfiniteList` of tree elements that corresponds to a given infinite address. -/
+def branchForAddress (t : PossiblyInfiniteTree α) (ns : InfiniteList Nat) : PossiblyInfiniteList α where
+  infinite_list := t.infinite_tree.branchForAddress ns
+  no_holes := by
+    intro n
+    rw [InfiniteTreeSkeleton.get_branchForAddress]
+    intro eq_none
+    rw [InfiniteTreeSkeleton.get_branchForAddress]
+    rw [InfiniteList.take_succ']
+    apply t.no_orphans
+    exact eq_none
+
+/-- An infinite address is maximal in a `PossiblyInfiniteTree` if whenever the the tree element is `none` at the nth step of the address, then all of its siblings are also none (and it is enough to demand that the first sibling is none). -/
+def branchAddressIsMaximal (t : PossiblyInfiniteTree α) (ns : InfiniteList Nat) : Prop :=
+  ∀ n, (t.branchForAddress ns).get? n.succ = none -> (t.drop (ns.take n)).childNodes.head = none
+
+/-- The `branches` in the `PossiblyInfiniteTree` are exactly the `PossiblyInfiniteList`s for which an infinite address exists that is also maximal. -/
+def branches (t : PossiblyInfiniteTree α) : Set (PossiblyInfiniteList α) :=
+  fun b => ∃ ns, b = t.branchForAddress ns ∧ t.branchAddressIsMaximal ns
+
+/-- Getting from the branch corresponding to an infinite address corresponds to getting from the tree at the corresponding finite part of the address. -/
+theorem get?_branchForAddress {t : PossiblyInfiniteTree α} {ns : InfiniteList Nat} {n : Nat} : (t.branchForAddress ns).get? n = t.get? (ns.take n) := by rfl
+
+/-- The set of `branches` can equivalently be expressed as the set of all `PossiblyInfiniteList`s where the head equals the root of the tree and the tail occurs in the branches of some childTree. If there are no childTrees, then the tail needs to be empty. -/
+theorem branches_eq {t : PossiblyInfiniteTree α} : t.branches = fun b =>
+    b.head = t.root ∧ ((t.childTrees = PossiblyInfiniteList.empty ∧ b.tail = PossiblyInfiniteList.empty) ∨ (∃ c ∈ t.childTrees, b.tail ∈ c.val.branches)) := by
+  unfold branches
+  apply Set.ext
+  intro b
+  constructor
+  . rintro ⟨ns, b_eq, ns_max⟩
+    constructor
+    . rw [b_eq]; rfl
+    . cases eq : t.childTrees.get? (ns.get 0) with
+      | none =>
+        apply Or.inl
+        rw [get?_childTrees] at eq
+        rw [PossiblyInfiniteTreeWithRoot.tree_to_opt_none_iff] at eq
+        rw [root_drop] at eq
+        rw [PossiblyInfiniteList.empty_iff_head_none]
+        rw [PossiblyInfiniteList.empty_iff_head_none]
         constructor
-        . apply PossiblyInfiniteList.ext
-          intro n
-          cases n with
-          | zero =>
-            rw [get?_branchForAddress, InfiniteList.take_zero]
-            exact head_eq
-          | succ n =>
-            rw [← PossiblyInfiniteList.get?_tail]
-            rw [tail_eq.right, PossiblyInfiniteList.get?_empty]
-            rw [get?_branchForAddress, InfiniteList.take_succ, ← List.singleton_append, ← get?_drop]
-            simp only [InfiniteList.head, InfiniteList.get]
-            have : t.childTrees.get? 0 = none := by rw [tail_eq.left, PossiblyInfiniteList.get?_empty]
-            rw [get?_childTrees, PossiblyInfiniteTreeWithRoot.tree_to_opt_none_iff] at this
-            rw [← empty_iff_root_none] at this
-            rw [this, get?_empty]
-        . intro n
-          rw [get?_branchForAddress, InfiniteList.take_succ', ← List.singleton_append, ← get?_drop]
-          simp only [InfiniteList.get, List.append_nil]
+        . specialize ns_max 0
+          rw [get?_branchForAddress] at ns_max
+          rw [InfiniteList.take_succ, InfiniteList.take_zero, InfiniteList.take_zero, drop_nil] at ns_max
+          unfold InfiniteList.head at ns_max
+          specialize ns_max eq
+          rw [PossiblyInfiniteList.head_eq] at ns_max
           rw [PossiblyInfiniteList.head_eq]
-          rw [get?_childNodes]
-          rw [← PossiblyInfiniteTreeWithRoot.opt_to_tree_none_iff]
-          rw [get?_childTrees]
-          rw [PossiblyInfiniteTreeWithRoot.tree_to_opt_none_iff]
-          rw [root_drop]
-          intro h; exact h
-      | inr tail_eq =>
-        rcases tail_eq with ⟨c, c_mem, ns, tail_eq, ns_max⟩
-        rw [PossiblyInfiniteList.mem_iff] at c_mem
-        rcases c_mem with ⟨i, c_mem⟩
-        exists InfiniteList.cons i ns
-        rw [get?_childTrees] at c_mem
-        rw [PossiblyInfiniteTreeWithRoot.tree_to_opt_some_iff] at c_mem
+          rw [get?_childNodes, ← PossiblyInfiniteTreeWithRoot.opt_to_tree_none_iff] at ns_max
+          exact ns_max
+        . rw [b_eq]
+          rw [PossiblyInfiniteList.head_eq, PossiblyInfiniteList.get?_tail]
+          rw [get?_branchForAddress]
+          rw [InfiniteList.take_succ, InfiniteList.take_zero]
+          unfold InfiniteList.head
+          exact eq
+      | some c =>
+        apply Or.inr
+        exists c
         constructor
-        . apply PossiblyInfiniteList.ext
+        . exists ns.get 0
+        exists ns.tail
+        rw [get?_childTrees] at eq
+        rw [PossiblyInfiniteTreeWithRoot.tree_to_opt_some_iff] at eq
+        constructor
+        . rw [b_eq]
+          apply PossiblyInfiniteList.ext
           intro n
+          rw [PossiblyInfiniteList.get?_tail]
           rw [get?_branchForAddress]
-          cases n with
-          | zero => rw [InfiniteList.take_zero]; exact head_eq
-          | succ n =>
-            rw [← PossiblyInfiniteList.get?_tail, tail_eq]
-            rw [InfiniteList.take_succ, InfiniteList.head_cons, InfiniteList.tail_cons]
-            rw [← List.singleton_append]
-            rw [← get?_drop]
-            rw [c_mem.left]
-            rw [get?_branchForAddress]
+          rw [get?_branchForAddress]
+          rw [InfiniteList.take_succ]
+          rw [← List.singleton_append]
+          rw [← get?_drop]
+          unfold InfiniteList.head
+          rw [eq.left]
         . intro n
+          specialize ns_max (n+1)
+          rw [get?_branchForAddress] at ns_max
+          rw [InfiniteList.take_succ] at ns_max
+          rw [← List.singleton_append] at ns_max
+          rw [← get?_drop] at ns_max
+          unfold InfiniteList.head at ns_max
+          rw [eq.left] at ns_max
           rw [get?_branchForAddress]
-          cases n with
-          | zero =>
-            intro contra
-            rw [InfiniteList.take_succ, InfiniteList.take_zero, InfiniteList.head_cons] at contra
-            rw [root_drop] at c_mem
-            rw [contra] at c_mem
-            simp at c_mem
-          | succ n =>
-            specialize ns_max n
-            rw [InfiniteList.take_succ, InfiniteList.head_cons, InfiniteList.tail_cons]
-            rw [← List.singleton_append]
-            rw [← get?_drop]
-            rw [c_mem.left]
-            rw [get?_branchForAddress] at ns_max
-            intro h; specialize ns_max h
-            rw [InfiniteList.take_succ, InfiniteList.head_cons, InfiniteList.tail_cons]
-            rw [← List.singleton_append]
-            rw [← drop_drop]
-            rw [c_mem.left]
-            exact ns_max
+          intro h
+          specialize ns_max h
+          rw [InfiniteList.take_succ] at ns_max
+          rw [← List.singleton_append] at ns_max
+          rw [← drop_drop] at ns_max
+          unfold InfiniteList.head at ns_max
+          rw [eq.left] at ns_max
+          exact ns_max
+  . rintro ⟨head_eq, tail_eq⟩
+    cases tail_eq with
+    | inl tail_eq =>
+      exists fun _ => 0
+      constructor
+      . apply PossiblyInfiniteList.ext
+        intro n
+        cases n with
+        | zero =>
+          rw [get?_branchForAddress, InfiniteList.take_zero]
+          exact head_eq
+        | succ n =>
+          rw [← PossiblyInfiniteList.get?_tail]
+          rw [tail_eq.right, PossiblyInfiniteList.get?_empty]
+          rw [get?_branchForAddress, InfiniteList.take_succ, ← List.singleton_append, ← get?_drop]
+          simp only [InfiniteList.head, InfiniteList.get]
+          have : t.childTrees.get? 0 = none := by rw [tail_eq.left, PossiblyInfiniteList.get?_empty]
+          rw [get?_childTrees, PossiblyInfiniteTreeWithRoot.tree_to_opt_none_iff] at this
+          rw [← empty_iff_root_none] at this
+          rw [this, get?_empty]
+      . intro n
+        rw [get?_branchForAddress, InfiniteList.take_succ', ← List.singleton_append, ← get?_drop]
+        simp only [InfiniteList.get, List.append_nil]
+        rw [PossiblyInfiniteList.head_eq]
+        rw [get?_childNodes]
+        rw [← PossiblyInfiniteTreeWithRoot.opt_to_tree_none_iff]
+        rw [get?_childTrees]
+        rw [PossiblyInfiniteTreeWithRoot.tree_to_opt_none_iff]
+        rw [root_drop]
+        intro h; exact h
+    | inr tail_eq =>
+      rcases tail_eq with ⟨c, c_mem, ns, tail_eq, ns_max⟩
+      rw [PossiblyInfiniteList.mem_iff] at c_mem
+      rcases c_mem with ⟨i, c_mem⟩
+      exists InfiniteList.cons i ns
+      rw [get?_childTrees] at c_mem
+      rw [PossiblyInfiniteTreeWithRoot.tree_to_opt_some_iff] at c_mem
+      constructor
+      . apply PossiblyInfiniteList.ext
+        intro n
+        rw [get?_branchForAddress]
+        cases n with
+        | zero => rw [InfiniteList.take_zero]; exact head_eq
+        | succ n =>
+          rw [← PossiblyInfiniteList.get?_tail, tail_eq]
+          rw [InfiniteList.take_succ, InfiniteList.head_cons, InfiniteList.tail_cons]
+          rw [← List.singleton_append]
+          rw [← get?_drop]
+          rw [c_mem.left]
+          rw [get?_branchForAddress]
+      . intro n
+        rw [get?_branchForAddress]
+        cases n with
+        | zero =>
+          intro contra
+          rw [InfiniteList.take_succ, InfiniteList.take_zero, InfiniteList.head_cons] at contra
+          rw [root_drop] at c_mem
+          rw [contra] at c_mem
+          simp at c_mem
+        | succ n =>
+          specialize ns_max n
+          rw [InfiniteList.take_succ, InfiniteList.head_cons, InfiniteList.tail_cons]
+          rw [← List.singleton_append]
+          rw [← get?_drop]
+          rw [c_mem.left]
+          rw [get?_branchForAddress] at ns_max
+          intro h; specialize ns_max h
+          rw [InfiniteList.take_succ, InfiniteList.head_cons, InfiniteList.tail_cons]
+          rw [← List.singleton_append]
+          rw [← drop_drop]
+          rw [c_mem.left]
+          exact ns_max
 
-  def generate_branch (start : Option β) (generator : β -> Option β) (mapper : β -> PossiblyInfiniteTreeWithRoot α) : PossiblyInfiniteList α :=
-    (PossiblyInfiniteList.generate start generator mapper).map (fun t => t.val.root.get (by rw [Option.isSome_iff_ne_none]; exact t.property))
+end Branches
 
-  theorem generate_branch_mem_branches {start : Option β} {generator : β -> Option β} {mapper : β -> PossiblyInfiniteTreeWithRoot α}
-      (next_is_child : ∀ b, ∀ b' ∈ generator b, mapper b' ∈ (mapper b).val.childTrees)
-      (maximal : ∀ b, generator b = none -> (mapper b).val.childTrees = PossiblyInfiniteList.empty)
-      (isSome_start : start.isSome) :
-      generate_branch start generator mapper ∈ (mapper (start.get isSome_start)).val.branches := by
-    let addresses : InfiniteList Nat := InfiniteList.generate start (fun o => o.bind generator)
-      (fun o => (o.bind (fun b => (generator b).attach.map (fun b' => Classical.choose (next_is_child b b'.val b'.property)))).getD 0)
-    let trees := PossiblyInfiniteList.generate start generator mapper
-    have : ∀ n, PossiblyInfiniteTreeWithRoot.opt_to_tree (trees.get? n) = (trees.head.get (by simp only [trees, PossiblyInfiniteList.head_generate, Option.isSome_map]; exact isSome_start)).val.drop (addresses.take n) := by
-      intro n
-      induction n with
-      | zero =>
-        simp only [InfiniteList.take_zero, drop_nil, PossiblyInfiniteList.head_eq, PossiblyInfiniteTreeWithRoot.opt_to_tree]
-        split
-        case h_1 _ eq => simp only [trees, ← PossiblyInfiniteList.head_eq, PossiblyInfiniteList.head_generate, Option.map_eq_none_iff] at eq; rw [eq] at isSome_start; simp at isSome_start
-        case h_2 _ _ eq => simp [eq]
-      | succ n ih =>
-        rw [InfiniteList.take_succ', ← drop_drop, ← ih]
-        cases eq : trees.get? n with
+section Generate
+
+/-!
+# Branch Generation
+
+We can use `PossiblyInfiniteList.generate` to construct `branches` in a `PossiblyInfiniteTree`.
+First of all, this requires that the mapper function produces a `PossiblyInfiniteTreeWithRoot`.
+By that `PossiblyInfiniteList.generate` gives us an `PossiblyInfiniteList` of `PossiblyInfiniteTreeWithRoot`.
+Intuitively, using all the roots of these trees gives us a branch.
+But this is only true if the generate trees are always child trees of each other and the generation indeed creates a maximal branch according to `branchAddressIsMaximal`.
+This condition is used in the `generate_branch_mem_branches` theorem to proof that a `PossiblyInfiniteList`
+from the `generate_branch` function is indeed in `branches`.
+-/
+
+/-- Given a generator and a mapper that maps generated elements to `PossiblyInfiniteTreeWithRoot`, construct an `PossiblyInfiniteList` with the goal of constructing a branch in a tree. -/
+def generate_branch (start : Option β) (generator : β -> Option β) (mapper : β -> PossiblyInfiniteTreeWithRoot α) : PossiblyInfiniteList α :=
+  (PossiblyInfiniteList.generate start generator mapper).map (fun t => t.val.root.get (by rw [Option.isSome_iff_ne_none]; exact t.property))
+
+/-- If the generated trees are `childTrees` of each other and the generated branch is maximal according to `branchAddressIsMaximal`, then the generated `PossiblyInfiniteList` is indeed a branch. -/
+theorem generate_branch_mem_branches {start : Option β} {generator : β -> Option β} {mapper : β -> PossiblyInfiniteTreeWithRoot α}
+    (next_is_child : ∀ b, ∀ b' ∈ generator b, mapper b' ∈ (mapper b).val.childTrees)
+    (maximal : ∀ b, generator b = none -> (mapper b).val.childTrees = PossiblyInfiniteList.empty)
+    (isSome_start : start.isSome) :
+    generate_branch start generator mapper ∈ (mapper (start.get isSome_start)).val.branches := by
+  let addresses : InfiniteList Nat := InfiniteList.generate start (fun o => o.bind generator)
+    (fun o => (o.bind (fun b => (generator b).attach.map (fun b' => Classical.choose (next_is_child b b'.val b'.property)))).getD 0)
+  let trees := PossiblyInfiniteList.generate start generator mapper
+  have : ∀ n, PossiblyInfiniteTreeWithRoot.opt_to_tree (trees.get? n) = (trees.head.get (by simp only [trees, PossiblyInfiniteList.head_generate, Option.isSome_map]; exact isSome_start)).val.drop (addresses.take n) := by
+    intro n
+    induction n with
+    | zero =>
+      simp only [InfiniteList.take_zero, drop_nil, PossiblyInfiniteList.head_eq, PossiblyInfiniteTreeWithRoot.opt_to_tree]
+      split
+      case h_1 _ eq => simp only [trees, ← PossiblyInfiniteList.head_eq, PossiblyInfiniteList.head_generate, Option.map_eq_none_iff] at eq; rw [eq] at isSome_start; simp at isSome_start
+      case h_2 _ _ eq => simp [eq]
+    | succ n ih =>
+      rw [InfiniteList.take_succ', ← drop_drop, ← ih]
+      cases eq : trees.get? n with
+      | none =>
+        conv => right; simp only [PossiblyInfiniteTreeWithRoot.opt_to_tree]
+        rw [drop_empty, empty_iff_root_none, ← PossiblyInfiniteTreeWithRoot.opt_to_tree_none_iff]
+        apply trees.no_holes'; exact eq
+      | some t =>
+        cases eq2 : trees.get? (n + 1) with
         | none =>
-          conv => right; simp only [PossiblyInfiniteTreeWithRoot.opt_to_tree]
-          rw [drop_empty, empty_iff_root_none, ← PossiblyInfiniteTreeWithRoot.opt_to_tree_none_iff]
-          apply trees.no_holes'; exact eq
-        | some t =>
-          cases eq2 : trees.get? (n + 1) with
-          | none =>
-            simp only [PossiblyInfiniteTreeWithRoot.opt_to_tree]
-            simp only [trees, PossiblyInfiniteList.get?_generate, Option.map_eq_some_iff] at eq
-            simp only [trees, PossiblyInfiniteList.get?_succ_generate, Option.map_eq_none_iff, Option.bind_eq_none_iff] at eq2
-            rcases eq with ⟨b, b_mem, eq⟩
-            specialize maximal b (eq2 b b_mem)
-            rw [eq] at maximal
-            have : PossiblyInfiniteTreeWithRoot.opt_to_tree (t.val.childTrees.get? (addresses.get n)) = empty := by
-              rw [maximal, PossiblyInfiniteList.get?_empty]; rfl
-            rw [get?_childTrees, PossiblyInfiniteTreeWithRoot.opt_to_tree_after_tree_to_opt] at this
-            rw [this]
-          | some t2 =>
-            simp only [trees, PossiblyInfiniteList.get?_generate, Option.map_eq_some_iff] at eq
-            simp only [trees, PossiblyInfiniteList.get?_succ_generate] at eq2
-            rcases eq with ⟨b, b_mem, eq⟩
-            rw [b_mem, Option.bind_some, Option.map_eq_some_iff] at eq2
-            rcases eq2 with ⟨b', b'_mem, t2_eq⟩
-            have eq_child := Classical.choose_spec (next_is_child b b' b'_mem)
-            rw [← t2_eq, ← eq_child]
-            conv => left; right; left; rw [eq]
-            rw [← PossiblyInfiniteList.get?.eq_def, get?_childTrees, PossiblyInfiniteTreeWithRoot.opt_to_tree_after_tree_to_opt]
-            simp only [PossiblyInfiniteTreeWithRoot.opt_to_tree]
-            have : addresses.get n = Classical.choose (next_is_child b b' b'_mem) := by
-              simp only [addresses, InfiniteList.get_generate]
-              rw [b_mem, Option.bind_some]
-              have : (generator b).attach = some ⟨b', b'_mem⟩ := by simp [b'_mem]
-              conv => left; left; right; rw [this]
-              rw [Option.map_some, Option.getD_some]
-            rw [this]
-    exists addresses; constructor
-    . apply PossiblyInfiniteList.ext
-      intro n
-      simp only [generate_branch]
-      rw [PossiblyInfiniteList.get?_map, get?_branchForAddress]
-      simp only [trees, PossiblyInfiniteList.head_generate, Option.get_map] at this
-      rw [← root_drop, ← this]
-      cases (PossiblyInfiniteList.generate start generator mapper).get? n <;> simp [PossiblyInfiniteTreeWithRoot.opt_to_tree, root_empty]
-    . intro n
-      rw [get?_branchForAddress]
-      simp only [trees, PossiblyInfiniteList.head_generate, Option.get_map] at this
-      rw [← root_drop, ← this, ← PossiblyInfiniteTreeWithRoot.opt_to_tree_none_iff]
-      rw [← this]
-      rw [PossiblyInfiniteList.get?_succ_generate, PossiblyInfiniteList.get?_generate, Option.map_eq_none_iff]
-      rw [PossiblyInfiniteList.head_eq, get?_childNodes, ← PossiblyInfiniteTreeWithRoot.opt_to_tree_none_iff, ← PossiblyInfiniteList.head_eq, ← PossiblyInfiniteList.empty_iff_head_none]
-      rw [Option.bind_eq_none_iff]
-      intro eq_none
-      cases b_eq : (InfiniteList.iterate start fun x => x.bind generator).get n with
-      | none => simp [PossiblyInfiniteTreeWithRoot.opt_to_tree, childTrees_empty]
-      | some b => simp only [Option.map_some, PossiblyInfiniteTreeWithRoot.opt_to_tree]; apply maximal; apply eq_none; exact b_eq
+          simp only [PossiblyInfiniteTreeWithRoot.opt_to_tree]
+          simp only [trees, PossiblyInfiniteList.get?_generate, Option.map_eq_some_iff] at eq
+          simp only [trees, PossiblyInfiniteList.get?_succ_generate, Option.map_eq_none_iff, Option.bind_eq_none_iff] at eq2
+          rcases eq with ⟨b, b_mem, eq⟩
+          specialize maximal b (eq2 b b_mem)
+          rw [eq] at maximal
+          have : PossiblyInfiniteTreeWithRoot.opt_to_tree (t.val.childTrees.get? (addresses.get n)) = empty := by
+            rw [maximal, PossiblyInfiniteList.get?_empty]; rfl
+          rw [get?_childTrees, PossiblyInfiniteTreeWithRoot.opt_to_tree_after_tree_to_opt] at this
+          rw [this]
+        | some t2 =>
+          simp only [trees, PossiblyInfiniteList.get?_generate, Option.map_eq_some_iff] at eq
+          simp only [trees, PossiblyInfiniteList.get?_succ_generate] at eq2
+          rcases eq with ⟨b, b_mem, eq⟩
+          rw [b_mem, Option.bind_some, Option.map_eq_some_iff] at eq2
+          rcases eq2 with ⟨b', b'_mem, t2_eq⟩
+          have eq_child := Classical.choose_spec (next_is_child b b' b'_mem)
+          rw [← t2_eq, ← eq_child]
+          conv => left; right; left; rw [eq]
+          rw [← PossiblyInfiniteList.get?.eq_def, get?_childTrees, PossiblyInfiniteTreeWithRoot.opt_to_tree_after_tree_to_opt]
+          simp only [PossiblyInfiniteTreeWithRoot.opt_to_tree]
+          have : addresses.get n = Classical.choose (next_is_child b b' b'_mem) := by
+            simp only [addresses, InfiniteList.get_generate]
+            rw [b_mem, Option.bind_some]
+            have : (generator b).attach = some ⟨b', b'_mem⟩ := by simp [b'_mem]
+            conv => left; left; right; rw [this]
+            rw [Option.map_some, Option.getD_some]
+          rw [this]
+  exists addresses; constructor
+  . apply PossiblyInfiniteList.ext
+    intro n
+    simp only [generate_branch]
+    rw [PossiblyInfiniteList.get?_map, get?_branchForAddress]
+    simp only [trees, PossiblyInfiniteList.head_generate, Option.get_map] at this
+    rw [← root_drop, ← this]
+    cases (PossiblyInfiniteList.generate start generator mapper).get? n <;> simp [PossiblyInfiniteTreeWithRoot.opt_to_tree, root_empty]
+  . intro n
+    rw [get?_branchForAddress]
+    simp only [trees, PossiblyInfiniteList.head_generate, Option.get_map] at this
+    rw [← root_drop, ← this, ← PossiblyInfiniteTreeWithRoot.opt_to_tree_none_iff]
+    rw [← this]
+    rw [PossiblyInfiniteList.get?_succ_generate, PossiblyInfiniteList.get?_generate, Option.map_eq_none_iff]
+    rw [PossiblyInfiniteList.head_eq, get?_childNodes, ← PossiblyInfiniteTreeWithRoot.opt_to_tree_none_iff, ← PossiblyInfiniteList.head_eq, ← PossiblyInfiniteList.empty_iff_head_none]
+    rw [Option.bind_eq_none_iff]
+    intro eq_none
+    cases b_eq : (InfiniteList.iterate start fun x => x.bind generator).get n with
+    | none => simp [PossiblyInfiniteTreeWithRoot.opt_to_tree, childTrees_empty]
+    | some b => simp only [Option.map_some, PossiblyInfiniteTreeWithRoot.opt_to_tree]; apply maximal; apply eq_none; exact b_eq
 
-  theorem head_generate_branch {start : Option β} {generator : β -> Option β} {mapper : β -> PossiblyInfiniteTreeWithRoot α} : (generate_branch start generator mapper).head = start.map (fun s => (mapper s).val.root.get (by rw [Option.isSome_iff_ne_none]; exact (mapper s).property)) := by simp only [generate_branch]; rw [PossiblyInfiniteList.head_eq, PossiblyInfiniteList.get?_map, ← PossiblyInfiniteList.head_eq, PossiblyInfiniteList.head_generate, Option.map_map]; rfl
+/-- The `PossiblyInfiniteList.head` of `generate_branch` is the `root` of the first tree. -/
+theorem head_generate_branch {start : Option β} {generator : β -> Option β} {mapper : β -> PossiblyInfiniteTreeWithRoot α} : (generate_branch start generator mapper).head = start.map (fun s => (mapper s).val.root.get (by rw [Option.isSome_iff_ne_none]; exact (mapper s).property)) := by simp only [generate_branch]; rw [PossiblyInfiniteList.head_eq, PossiblyInfiniteList.get?_map, ← PossiblyInfiniteList.head_eq, PossiblyInfiniteList.head_generate, Option.map_map]; rfl
 
-  theorem get?_generate_branch {start : Option β} {generator : β -> Option β} {mapper : β -> PossiblyInfiniteTreeWithRoot α} :
-    ∀ n, (generate_branch start generator mapper).get? n = ((PossiblyInfiniteList.generate start generator mapper).get? n).map (fun t => t.val.root.get (by rw [Option.isSome_iff_ne_none]; exact t.property)) := by intros; rfl
+/-- Getting the nth element from a `generate_branch` result is the root of the nth generated tree. -/
+theorem get?_generate_branch {start : Option β} {generator : β -> Option β} {mapper : β -> PossiblyInfiniteTreeWithRoot α} :
+  ∀ n, (generate_branch start generator mapper).get? n = ((PossiblyInfiniteList.generate start generator mapper).get? n).map (fun t => t.val.root.get (by rw [Option.isSome_iff_ne_none]; exact t.property)) := by intros; rfl
 
-  theorem tail_generate_branch {start : Option β} {generator : β -> Option β} {mapper : β -> PossiblyInfiniteTreeWithRoot α} : (generate_branch start generator mapper).tail = generate_branch (start.bind generator) generator mapper := by unfold generate_branch; rw [PossiblyInfiniteList.tail_map, PossiblyInfiniteList.tail_generate]
+/-- The `PossiblyInfiniteList.tail` of `generate_branch` is the branch generated when applying the generator function once on the starting element before the actual generation. -/
+theorem tail_generate_branch {start : Option β} {generator : β -> Option β} {mapper : β -> PossiblyInfiniteTreeWithRoot α} : (generate_branch start generator mapper).tail = generate_branch (start.bind generator) generator mapper := by unfold generate_branch; rw [PossiblyInfiniteList.tail_map, PossiblyInfiniteList.tail_generate]
 
-  def leaves (t : PossiblyInfiniteTree α) : Set α := fun a => ∃ node : List Nat, t.get? node = some a ∧ (t.drop node).childNodes.head = none
+end Generate
 
-  def from_branch (b : PossiblyInfiniteList α) : PossiblyInfiniteTree α where
-    infinite_tree := fun ns => if ns.all (fun e => e = 0) then b.infinite_list ns.length else none
-    no_orphans := by
-      intro ns eq_none n
-      simp only [InfiniteTreeSkeleton.get] at eq_none
-      rw [InfiniteTreeSkeleton.get_childNodes, InfiniteTreeSkeleton.get_drop]
-      simp only [InfiniteTreeSkeleton.get]
-      cases eq : (ns ++ [n]).all (fun e => e = 0) with
-      | false => rfl
-      | true =>
-        have : ns.all (fun e => e = 0) := by rw [List.all_append, Bool.and_eq_true] at eq; exact eq.left
-        simp only [this] at eq_none
-        simp only [List.length_append, List.length_singleton]
-        apply b.no_holes
-        exact eq_none
-    no_holes_in_children := by
-      rintro _ ⟨ns, eq⟩ n _
-      rw [← eq, InfiniteTreeSkeleton.get_childNodes, InfiniteTreeSkeleton.get_drop]
-      simp only [InfiniteTreeSkeleton.get]
-      have : (ns ++ [n.succ]).all (fun e => e = 0) = false := by
-        rw [List.all_eq_false]
-        exists n.succ
-        simp
-      simp [this]
+section Leaves
+
+/-!
+## Leaves
+
+The `leaves` of a `PossiblyInfiniteTree` is the set of elements that occur in a node that has no `childNodes`.
+-/
+
+def leaves (t : PossiblyInfiniteTree α) : Set α := fun a => ∃ node : List Nat, t.get? node = some a ∧ (t.drop node).childNodes.head = none
+
+end Leaves
+
+section FromBranch
+
+/-!
+## Constructing a Tree from a Branch
+
+A `PossiblyInfiniteList` directly corresponds to the `PossiblyInfiniteTree`
+where the list is the "first" branch (with the address that only consists of zeros) and all other nodes are none.
+-/
+
+def from_branch (b : PossiblyInfiniteList α) : PossiblyInfiniteTree α where
+  infinite_tree := fun ns => if ns.all (fun e => e = 0) then b.infinite_list ns.length else none
+  no_orphans := by
+    intro ns eq_none n
+    simp only [InfiniteTreeSkeleton.get] at eq_none
+    rw [InfiniteTreeSkeleton.get_childNodes, InfiniteTreeSkeleton.get_drop]
+    simp only [InfiniteTreeSkeleton.get]
+    cases eq : (ns ++ [n]).all (fun e => e = 0) with
+    | false => rfl
+    | true =>
+      have : ns.all (fun e => e = 0) := by rw [List.all_append, Bool.and_eq_true] at eq; exact eq.left
+      simp only [this] at eq_none
+      simp only [List.length_append, List.length_singleton]
+      apply b.no_holes
+      exact eq_none
+  no_holes_in_children := by
+    rintro _ ⟨ns, eq⟩ n _
+    rw [← eq, InfiniteTreeSkeleton.get_childNodes, InfiniteTreeSkeleton.get_drop]
+    simp only [InfiniteTreeSkeleton.get]
+    have : (ns ++ [n.succ]).all (fun e => e = 0) = false := by
+      rw [List.all_eq_false]
+      exists n.succ
+      simp
+    simp [this]
+
+end FromBranch
 
 end PossiblyInfiniteTree
 
